HITs/ntrunc.lean
@@ -6,6 +6,8 @@ open ground_zero.HITs.ncircle (S)
 namespace ground_zero
 namespace HITs
 
+local infix ` = ` := eq
+
 inductive {u} ntrunc.core (α : Sort u) : ℕ → Sort (u + 1)
 | elem {n : ℕ} : α → ntrunc.core n
 | hub {n : ℕ} : (S (n + 1) → ntrunc.core n) → ntrunc.core n
@@ -15,34 +17,28 @@ inductive {u} ntrunc.rel (α : Sort u) (n : ℕ) :
 | spoke (r : S (n + 1) → ntrunc.core α n) (x : S (n + 1)) :
   ntrunc.rel (r x) (ntrunc.core.hub r)
 
-def {u} ntrunc (n : homotopy_level) (α : Sort u) :=
-match n with
-| homotopy_level.minus_two := ground_zero.unit
-| homotopy_level.succ n :=
-  @quot (ntrunc.core α (homotopy_level.succ n))
-        (ntrunc.rel α (homotopy_level.succ n))
-end
+def {u} ntrunc (n : ℕ) (α : Sort u) :=
+@quot (ntrunc.core α n) (ntrunc.rel α n)
 
-def strunc := ntrunc 0
+def strunc := ntrunc 1
 notation `∥` α `∥₀` := strunc α
+
+namespace strunc
+  universe u
+
+  def elem {α : Sort u} (a : α) : ∥α∥₀ :=
+  quot.mk (ntrunc.rel α 1) (core.elem a)
+end strunc
 
 namespace ntrunc
   universe u
 
-  def elem {α : Sort u} {n : homotopy_level} (a : α) :
+  def elem {α : Sort u} {n : ℕ} (a : α) :
     ntrunc n α :=
-  match n with
-  | homotopy_level.minus_two := ground_zero.unit.star
-  | homotopy_level.succ n :=
-    quot.mk (rel α (homotopy_level.succ n)) (core.elem a)
-  end
+  quot.mk (rel α n) (core.elem a)
 
-  theorem truncation_is_correct {α : Sort u} {n : homotopy_level} :
-    is_n_type (ntrunc n α) n := begin
-    induction n with n ih,
-    { unfold is_n_type, simp [ntrunc],
-      apply contr.mk ground_zero.unit.star,
-      intro x, induction x, reflexivity },
+  theorem truncation_is_correct {α : Sort u} {n : ℕ} :
+    is_n_type (ntrunc n α) (n_to_level n) := begin
     admit
   end
 end ntrunc
